theories/Homomorphism.v
@@ -1,0 +1,50 @@
+From Coq Require Import String.
+From Hammer Require Import Tactics.
+From LambdaST Require Import
+  Context
+  Environment
+  FV
+  Hole
+  Derivative
+  Ind
+  Inert
+  Nullable
+  Prefix
+  Semantics
+  SinkTerm
+  Sets
+  Terms
+  Types
+  PrefixConcat
+  Subcontext
+  SemSound
+  Typing.
+
+Definition P_hom g (e : term) (s : type) (i : inertness) eta (e' : term) p :=
+  WFContext g ->
+  EnvTyped eta g ->
+  forall eta' eta'' e'' p' p'',
+  Step eta' e' e'' p' ->
+  PrefixConcat p p' p'' ->
+  EnvConcat eta eta' eta'' ->
+  Step eta'' e e'' p''
+.
+
+Theorem hom : forall g e s i eta e' p,
+    Typed g e s i ->
+    Step eta e e' p ->
+    P_hom g e s i eta e' p
+.
+Proof.
+apply (lex_ind P_hom); unfold P_hom in *; intros.
+- eapply H2. eapply subtcontext_wf; eauto. eapply sub_preserves_env; eauto. eauto. eauto. eauto.
+- best.
+- sinvert H3; unfold EnvConcat in *; econstructor; qauto l: on use:pfx_cat_unique.
+- sauto lq: on rew: off.
+- sinvert H5. sinvert H7. sinvert H8. sinvert H6.
+  + econstructor. hauto l: on. qauto l: on use:pfx_cat_maximal.
+  + sinvert H8. sinvert H6. econstructor; [ eauto | best use:pfx_cat_maximal |].
+    
+-
+intros.
+Admitted.
