theories/Ind.v
@@ -17,62 +17,33 @@ From LambdaST Require Import
   Inert
   Typing.
 
+Check Step_ind.
+Check Typed_ind.
+
 (*
-Typed_ind
-	 : forall P : context -> term -> type -> Prop,
-        ->
-        ->
-       (forall (G D : context) (e1 e2 : term) (s t : type),
-        Typed G e1 s ->
-        P G e1 s ->
-        Typed D e2 t ->
-        P D e2 t -> P (CtxSemic G D) (TmSemic e1 e2) (TyDot s t)) ->
-       (forall (G : hole) (x y z : string) (s t : type) 
-          (e : term) (r : type) (Gxsyt Gzst : context),
-        x <> y ->
-        ~ fv G x ->
-        ~ fv G y ->
-        Fill G (CtxSemic (CtxHasTy x s) (CtxHasTy y t)) Gxsyt ->
-        Fill G (CtxHasTy z (s . t)) Gzst ->
-        Typed Gxsyt e r -> P Gxsyt e r -> P Gzst (TmLetCat t x y z e) r) ->
-       (forall G : context, P G TmSink TyEps) ->
-       (forall G : context, P G TmUnit TyOne) ->
-       (forall (G : hole) (x : string) (s : type) (Gxs : context),
-        Fill G (CtxHasTy x s) Gxs -> P Gxs (TmVar x) s) ->
-       (forall (G G' : context) (e : term) (s : type),
-        Subcontext G G' -> Typed G' e s -> P G' e s -> P G e s) ->
-       (forall (G : hole) (D : context) (x : string) 
-          (e e' : term) (s t : type) (Gxs GD : context),
-        ~ fv G x ->
-        Typed D e s ->
-        P D e s ->
-        Fill G (CtxHasTy x s) Gxs ->
-        Fill G D GD -> Typed Gxs e' t -> P Gxs e' t -> P GD (TmLet x e e') t) ->
-       (forall (G : hole) (x : string) (s t : type) 
-          (e : term) (Ge Gxs : context),
-        Fill G CtxEmpty Ge ->
-        Fill G (CtxHasTy x s) Gxs ->
-        Typed Ge e t -> P Ge e t -> P Gxs (TmDrop x e) t) ->
-       forall (c : context) (t : term) (t0 : type), Typed c t t0 -> P c t t0
+
 Step_ind
 	 : forall P : env -> term -> term -> prefix -> Prop,
        (forall n : env, P n TmSink TmSink PfxEpsEmp) ->
        (forall n : env, P n TmUnit TmSink PfxOneFull) ->
        (forall (n : string -> option prefix) (x : string) (p : prefix),
         n x = Some p -> P n (TmVar x) (TmVar x) p) ->
-        ->
-       (forall (n : env) (e1 e1' e2 : term) (p : prefix),
-        Step n e1 e1' p ->
-        P n e1 e1' p ->
-        ~ MaximalPrefix p ->
-        P n (TmSemic e1 e2) (TmSemic e1' e2) (PfxCatFst p)) ->
        (forall (n : env) (e1 e1' e2 e2' : term) (p1 p2 : prefix),
         Step n e1 e1' p1 ->
         P n e1 e1' p1 ->
-        MaximalPrefix p1 ->
         Step n e2 e2' p2 ->
-        P n e2 e2' p2 -> P n (TmSemic e1 e2) e2' (PfxCatBoth p1 p2)) ->
+        P n e2 e2' p2 ->
+        P n (TmComma e1 e2) (TmComma e1' e2') (PfxParPair p1 p2)) ->
         ->
+        ->
+       (forall (n : string -> option prefix) (x y z : string) 
+          (e e' : term) (p1 p2 p' : prefix),
+        n z = Some (PfxParPair p1 p2) ->
+        Step
+          (env_union n (env_union (singleton_env x p1) (singleton_env y p2)))
+          e e' p' ->
+        P (env_union n (env_union (singleton_env x p1) (singleton_env y p2)))
+          e e' p' -> P n (TmLetPar x y z e) (TmLetPar x y z e') p') ->
        (forall (t : type) (n : string -> option prefix) 
           (x y z : string) (e e' : term) (p p' : prefix),
         n z = Some (PfxCatFst p) ->
@@ -92,7 +63,8 @@ Step_ind
           e e' p' ->
         P (env_union n (env_union (singleton_env x p1) (singleton_env y p2)))
           e e' p' ->
-        P n (TmLetCat t x y z e) (TmLet x (sink_tm p1) (subst_var e z y)) p') ->
+        P n (TmLetCat t x y z e)
+          (TmLet x (sink_tm p1) (Subst.subst_var e z y)) p') ->
        (forall (eta : env) (x : string) (e1 e2 e1' e2' : term)
           (p p' : prefix),
         Step eta e1 e1' p ->
@@ -100,14 +72,61 @@ Step_ind
         Step (env_subst x p eta) e2 e2' p' ->
         P (env_subst x p eta) e2 e2' p' ->
         P eta (TmLet x e1 e2) (TmLet x e1' e2') p') ->
-       (forall (eta : env) (x : string) (e e' : term) (p : prefix),
-        Step (env_drop eta x) e e' p ->
-        P (env_drop eta x) e e' p -> P eta (TmDrop x e) (TmDrop x e') p) ->
        forall (e : env) (t t0 : term) (p : prefix),
        Step e t t0 p -> P e t t0 p
 
 
 *)
+
+(*
+Typed_ind
+	 : forall P : context -> term -> type -> inertness -> Prop,
+       (forall (G : context) (e1 e2 : term) (s t : type)
+          (i1 i2 i3 : inertness),
+        Typed G e1 s i1 ->
+        P G e1 s i1 ->
+        Typed G e2 t i2 ->
+        P G e2 t i2 -> i_ub i1 i2 i3 -> P G (TmComma e1 e2) (TyPar s t) i3) ->
+       (forall (G : hole) (x y z : string) (s t : type) 
+          (e : term) (r : type) (Gxsyt Gzst : context) 
+          (i : inertness),
+        x <> y ->
+        ~ fv G x ->
+        ~ fv G y ->
+        Fill G (CtxComma (CtxHasTy x s) (CtxHasTy y t)) Gxsyt ->
+        Fill G (CtxHasTy z (s || t)) Gzst ->
+        Typed Gxsyt e r i -> P Gxsyt e r i -> P Gzst (TmLetPar x y z e) r i) ->
+        ->
+       (forall (G : hole) (x y z : string) (s t : type) 
+          (e : term) (r : type) (Gxsyt Gzst : context) 
+          (i : inertness),
+        x <> y ->
+        ~ fv G x ->
+        ~ fv G y ->
+        Fill G (CtxSemic (CtxHasTy x s) (CtxHasTy y t)) Gxsyt ->
+        Fill G (CtxHasTy z (s . t)) Gzst ->
+        Typed Gxsyt e r i -> P Gxsyt e r i -> P Gzst (TmLetCat t x y z e) r i) ->
+       (forall (G : context) (i : inertness), P G TmSink TyEps i) ->
+       (forall G : context, P G TmUnit TyOne Jumpy) ->
+       (forall (G : hole) (x : string) (s : type) 
+          (Gxs : context) (i : inertness),
+        Fill G (CtxHasTy x s) Gxs -> P Gxs (TmVar x) s i) ->
+       (forall (G G' : context) (e : term) (s : type) (i : inertness),
+        Subcontext G G' -> Typed G' e s i -> P G' e s i -> P G e s i) ->
+       (forall (G : hole) (D : context) (x : string) 
+          (e e' : term) (s t : type) (Gxs GD : context) 
+          (i : inertness),
+        ~ fv G x ->
+        Typed D e s Inert ->
+        P D e s Inert ->
+        Fill G (CtxHasTy x s) Gxs ->
+        Fill G D GD ->
+        Typed Gxs e' t i -> P Gxs e' t i -> P GD (TmLet x e e') t i) ->
+       forall (c : context) (t : term) (t0 : type) (i : inertness),
+       Typed c t t0 i -> P c t t0 i
+
+*)
+
 
 
 
@@ -139,6 +158,35 @@ Theorem lex_ind :
         forall IHe2 : P G e2 t i2 n e2' p2,
 
         P G (TmComma e1 e2) (TyPar s t) i3 n (TmComma e1' e2') (PfxParPair p1 p2)) ->
+
+    (* (forall (G D : context) (e1 e2 : term) (s t : type) (i1 i2 i3 : inertness),
+        Typed G e1 s i1 ->
+        P G e1 s i1 ->
+        Typed D e2 t i2 ->
+        P D e2 t i2 ->
+        inert_guard (i1 = Inert /\ ~ Nullable s) i3 ->
+        P (CtxSemic G D) (TmSemic e1 e2) (TyDot s t) i3) -> *)
+
+    (forall G D s t i1 i2 i3 (n : env) (e1 e1' e2 : term) (p : prefix),
+        Typed G e1 s i1 ->
+        Typed D e2 t i2 ->
+        inert_guard (i1 = Inert /\ ~ Nullable s) i3 ->
+        Step n e1 e1' p ->
+        P G e1 s i1 n e1' p ->
+        (~ MaximalPrefix p) ->
+        P (CtxSemic G D) (TmSemic e1 e2) (TyDot s t) i3 n (TmSemic e1' e2) (PfxCatFst p)
+      ) ->
+
+    (forall G D s t i1 i2 i3 (n : env) (e1 e1' e2 e2' : term) (p1 p2 : prefix),
+        Typed G e1 s i1 ->
+        Typed D e2 t i2 ->
+        inert_guard (i1 = Inert /\ ~ Nullable s) i3 ->
+        Step n e1 e1' p1 ->
+        P G e1 s i1 n e1' p1 ->
+        MaximalPrefix p1 ->
+        Step n e2 e2' p2 ->
+        P D e2 t i2 n e2' p2 ->
+        P (CtxSemic G D) (TmSemic e1 e2) (TyDot s t) i3 n e2' (PfxCatBoth p1 p2)) ->
     
     (forall G Gxsyt Gzst x y z s t r e n e' p1 p2 p' i,
 
@@ -162,7 +210,15 @@ Proof.
   intros.
   generalize dependent G.
   generalize dependent s.
-  induction H5; intros s G H00; admit.
+  generalize dependent i.
+  induction H7; intros s G i H00.
+  - admit.
+  - admit.
+  - admit.
+  - admit.
+  - dependent induction H00.
+    + hauto l: on.
+    + sfirstorder.
   (* - dependent induction H00; sfirstorder.
   - admit.
   - dependent induction H00; sfirstorder.
